\documentclass[../Summary.tex]{subfiles}

\begin{document}

\subsubsection{Summary}

\[
\begin{array}{lcrcl} 
\propname{TR}(S,\ \leq) \wedge \propname{AY}(S,\ \leq) \wedge \propname{LM}(S,\ \otimes,\ \leq)
	& \Rightarrow
	& \propname{LD}(\mathcal{N}(S,\ \otimes,\ \leq)) 
    & \Leftrightarrow 
    & \propname{TRUE}
    \\ 
\propname{TR}(S,\ \leq) \wedge \propname{AY}(S,\ \leq) \wedge \propname{RM}(S,\ \otimes,\ \leq)
	& \Rightarrow
	& \propname{RD}(\mathcal{N}(S,\ \otimes,\ \leq)) 
    & \Leftrightarrow 
    & \propname{TRUE}
    \\ 
& & \propname{ZA}(\mathcal{N}(S,\ \otimes,\ \leq)) 
    & \Leftrightarrow 
    & \propname{TRUE}
    \\ 
\propname{AY}(S,\leq) \wedge \propname{BM}(S,\leq) \wedge \propname{ID}(S,\otimes) \ \wedge \\
\ \ (\propname{LI}(S,\ \leq,\ \otimes) \vee \propname{RI}(S,\ \leq,\ \otimes) \ \vee \\
\ \ \propname{LM}(S,\ \leq,\ \otimes) \vee \propname{RM}(S,\ \leq,\ \otimes))
	& \Rightarrow 
	& \propname{OA}(\mathcal{N}(S,\ \otimes,\ \leq)) 
    & \Leftrightarrow 
    & \propname{TRUE}
    \\ 
\propname{TR}(S,\ \leq) \wedge \propname{AY}(S,\ \leq) \wedge \propname{LI}(S,\ \otimes,\ \leq) 
	& \Rightarrow 
	& \propname{LAB}(\mathcal{N}(S,\ \otimes,\ \leq)) 
    & \Leftrightarrow 
    & \propname{TRUE}
    \\ 
\propname{TR}(S,\ \leq) \wedge \propname{AY}(S,\ \leq) \wedge \propname{RI}(S,\ \otimes,\ \leq) 
	& \Rightarrow 
	& \propname{RAB}(\mathcal{N}(S,\ \otimes,\ \leq)) 
    & \Leftrightarrow 
    & \propname{TRUE}
    \\
\end{array} 
\] 

Lemmas and results used here can be found in the documentation for MinUnion ($\minunion$) and MinTimes ($\minlift$) respectively.



\subsubsection{Left distributive}

$\propname{LM}(S,\ \otimes,\ \leq) \wedge \propname{TR}(S,\ \otimes,\ \leq) \wedge \propname{AY}(S,\ \otimes, \ \leq) \Rightarrow (\propname{LD}(\mathcal{N}(S,\ \otimes,\ \leq))  \Leftrightarrow \propname{TRUE})$

\proof

Consider arbitrary $X,Y,Z$
\begin{align*}
X \minlift (Y \minunion Z) 	& = \min_\leq(X \lift \min_\leq(Y \cup Z)) \\
							& = \min_\leq(X \lift (Y \cup Z)) \\
							& = \min_\leq((X \lift Y) \cup (X \lift Z)) \\
							& = \min_\leq(\min_\leq(X \lift Y) \cup \min_\leq(X \lift Z)) \\
							& = (X \minlift Y) \minunion (X \minlift Z)
\end{align*}



\subsubsection{Right distributive}

$\propname{RM}(S,\ \otimes,\ \leq) \wedge \propname{TR}(S,\ \otimes,\ \leq) \wedge \propname{AY}(S,\ \otimes, \ \leq) \Rightarrow (\propname{RD}(\mathcal{N}(S,\ \otimes,\ \leq))  \Leftrightarrow \propname{TRUE})$

\proof

Consider arbitrary $X,Y,Z$
\begin{align*}
(X \minunion Y) \minlift Z 	& = \min_\leq(\min_\leq(X \cup Y) \ \lift \ Z) \\
							& = \min_\leq((X \cup Y) \ \lift \ Z) \\
							& = \min_\leq((X \lift Z) \cup (Y \lift Z)) \\
							& = \min_\leq(\min_\leq(X \lift Z) \cup \min_\leq(Y \lift Z)) \\
							& = (X \minlift Z) \minunion (Y \minlift Z)
\end{align*}



\subsubsection{Zero annihilates}

$\propname{ZA}(\mathcal{N}(S,\ \otimes,\ \leq)) \Leftrightarrow \propname{TRUE}$

\proof

Witness : $\emptyset$

\vspace{0.5em}

See MinUnion and MinLift documentation for details.



\subsubsection{One annihilates}

$\propname{AY}(S,\leq) \wedge \propname{BM}(S,\leq) \wedge \propname{ID}(S,\otimes) \wedge (\propname{LI}(S,\ \leq,\ \otimes) \vee \propname{RI}(S,\ \leq,\ \otimes) \vee \propname{LM}(S,\ \leq,\ \otimes) \vee \propname{RM}(S,\ \leq,\ \otimes)) \Rightarrow (\propname{OA}(\mathcal{N}(S,\ \otimes,\ \leq)) \Leftrightarrow \propname{TRUE})$

\proof

From $\propname{AY}(S,\leq)$ and $\propname{BM}(S,\leq)$ we have that $\{ \bot \}$ is an annihilator for $\minunion$ (see MinUnion documentation).

\vspace{0.5em}

From $\propname{ID}(S,\otimes)$ we have that $\{ i \}$ is an identity for $\minlift$ (see MinLift documentation).

\vspace{0.5em}

It remains to prove that $i = \bot$. Any of the four remaining properties suffice to show this. 

\vspace{0.5em}

For example assume $\propname{LM}(S,\ \leq,\ \otimes)$. Using this with $\propname{ID}(S,\otimes)$, we therefore have that:
\begin{align*}
i 	& = i \otimes i \\
  	& \leq i \otimes \bot \\
  	& = \bot
\end{align*} 
and by $\propname{BM}(S,\leq)$ we have that:
\begin{equation*}
\bot \leq i
\end{equation*}
Therefore by $\propname{AY}(S,\leq)$ we have that $i = \bot$.



\subsubsection{Left absorptive}

$\propname{TR}(S,\ \leq) \wedge \propname{AY}(S,\ \leq) \wedge \propname{LI}(S,\ \otimes,\ \leq) \Rightarrow (\propname{LAB}(\mathcal{N}(S,\ \otimes,\ \leq)) \Leftrightarrow \propname{TRUE})$

\proof

Consider arbitrary $X, Y$
\begin{align*}
X \minunion (X \minlift Y) 	& = \min_\leq(X \cup \min_\leq(X \lift Y)) \\
							& = \min_\leq(X \cup (X \lift Y)) \\
							& = \min_\leq(X) \\
							& = X
\end{align*}
The second equality holds by the commutativity of $\cup$.



\subsubsection{Right absorptive}

$\propname{TR}(S,\ \leq) \wedge \propname{AY}(S,\ \leq) \wedge \propname{RI}(S,\ \otimes,\ \leq) \Rightarrow (\propname{RAB}(\mathcal{N}(S,\ \otimes,\ \leq)) \Leftrightarrow \propname{TRUE})$

\proof

Consider arbitrary $X, Y$
\begin{align*}
X \minunion (Y \minlift X) 	& = \min_\leq(X \cup \min_\leq(Y \lift X)) \\
							& = \min_\leq(X \cup (Y \lift X)) \\
							& = \min_\leq(X) \\
							& = X	
\end{align*}
The second equality holds by the commutativity of $\cup$.

\end{document}