\documentclass[../Summary.tex]{subfiles}

\begin{document}

\subsubsection{Summary}

Assume $(S,\ \leq)$ is a pre-order.

\[
\begin{array}{lcrcl} 
\propname{TRUE}
	& \Rightarrow
	& \propname{AS}(\mathrm{MinUnion}(S, \leq)) 
	& \Leftrightarrow 
	& \propname{TRUE} 
	\\ 
\propname{TRUE}
	& \Rightarrow
	& \propname{ID}(\mathrm{MinUnion}(S, \leq)) 
	& \Leftrightarrow 
	& \propname{TRUE}
	\\
\propname{AY}(S, \leq) \wedge \propname{BM}(S, \leq)
	& \Rightarrow
	& \propname{AN}(\mathrm{MinUnion}(S, \leq)) 
	& \Leftrightarrow 
	& \propname{TRUE}
	\\
\propname{TRUE}
	& \Rightarrow
	& \propname{CM}(\mathrm{MinUnion}(S, \leq)) 
	& \Leftrightarrow 
  	& \propname{TRUE}
	\\ 
\propname{TRUE}
	& \Rightarrow
	& \propname{SL}(\mathrm{MinUnion}(S, \leq)) 
	& \Leftrightarrow 
	& \propname{TO}(S, \leq)  
	\\ 
\propname{TRUE}
	& \Rightarrow
	& \propname{IP}(\mathrm{MinUnion}(S, \leq)) 
	& \Leftrightarrow 
	& \propname{TRUE}
	\\ 
\propname{TRUE}
	& \Rightarrow
	& \propname{IL}(\mathrm{MinUnion}(S, \leq)) 
	& \Leftrightarrow
	& \propname{FALSE} 
	\\
\propname{TRUE}
	& \Rightarrow
	& \propname{IR}(\mathrm{MinUnion}(S, \leq)) 
	& \Leftrightarrow
	& \propname{FALSE} 
	\\
\propname{TRUE}
	& \Rightarrow
	& \propname{LC}(\mathrm{MinUnion}(S, \leq)) 
	& \Leftrightarrow
	& \propname{FALSE} 
	\\
\propname{TRUE}
	& \Rightarrow
	& \propname{RC}(\mathrm{MinUnion}(S, \leq)) 
	& \Leftrightarrow
	& \propname{FALSE} 
	\\
\propname{TRUE}
	& \Rightarrow
	& \propname{LK}(\mathrm{MinUnion}(S, \leq)) 
	& \Leftrightarrow
	& \propname{FALSE} 
	\\
\propname{TRUE}
	& \Rightarrow
	& \propname{RK}(\mathrm{MinUnion}(S, \leq)) 
	& \Leftrightarrow
	& \propname{FALSE} 
	\\
\propname{TRUE}
	& \Rightarrow
	& \propname{AL}(\mathrm{MinUnion}(S, \leq))  
	& \Leftrightarrow
	& \propname{FALSE} 
	\\
\propname{TRUE}
	& \Rightarrow
	& \propname{AR}(\mathrm{MinUnion}(S, \leq))  
	& \Leftrightarrow
	& \propname{FALSE} 
	\\
\end{array} 
\] 




\subsubsection{Useful lemmas}

\begin{lemma} \label{lem:minunion_left_absorption}
For all X and Y:
\begin{equation*}
\min_\leq(X \cup Y) = \min_\leq(\min_\leq(X) \cup Y)
\end{equation*}
\end{lemma}

\begin{proof}
Assume $z \in \min_\leq(X \cup Y)$. 
\begin{ind}
Then we have:
\begin{equation}
z \in X \ \vee \ z \in Y
\end{equation}
\begin{equation} \label{eq:lem_abs_minset_left_X}
\forall x \in X : \neg (x < z)
\end{equation}
\begin{equation} \label{eq:lem_abs_minset_left_Y}
\forall y \in Y : \neg (y < z)
\end{equation}

By Eq~\ref{eq:lem_abs_minset_left_Y} and the fact that $\min_\leq(Y) \subseteq Y$, we have that
\begin{equation*} 
\forall y \in \min_\leq(Y) : \neg (y < z)
\end{equation*}
and combining this with Eq~\ref{eq:lem_abs_minset_left_X} gives
\begin{equation} \label{eq:lem_abs_minset_left_XminsetY}
\forall x \in X \cup \min_\leq(Y) : \neg (x < z)
\end{equation}

Case $z \in X$
\begin{ind}
Clearly $z \in X \, \cup \, \min_\leq(Y)$ and by combining this with Eq~\ref{eq:lem_abs_minset_left_XminsetY} we have that $x \in \min_\leq(X \cup \min_\leq(Y))$.
\end{ind}

Case $z \in Y$
\begin{ind}
By Eq~\ref{eq:lem_abs_minset_left_Y} we have that $z \in \min_\leq(Y)$ and hence we have that $z \in X \cup \min_\leq(Y)$. By Eq \ref{eq:lem_abs_minset_left_XminsetY} we have that $z \in \min_\leq(X \cup \min_\leq(Y))$.
\end{ind}

Hence $z \in \min_\leq(X \cup Y) \Rightarrow z \in \min_\leq(X \cup \min_\leq(Y))$.
\end{ind}

\vspace{2em}

Assume $z \in \min_\leq(X \cup \min_\leq(Y))$.

\begin{ind}
Then we have:
\begin{equation}
z \in X \ \vee \ z \in \min_\leq(Y)
\end{equation}
\begin{equation} \label{eq:lem_abs_minset_right_X}
\forall x \in X : \neg (x < z)
\end{equation}
\begin{equation} \label{eq:lem_abs_minset_right_minsetY}
\forall y \in \min_\leq(Y) : \neg (y < z)
\end{equation}

Assume $\exists w \in Y : y < w$
\begin{ind}
Clearly $w \notin \min_\leq(Y)$ otherwise Eq~\ref{eq:lem_abs_minset_right_minsetY} would be contradicted. Therefore by definition of $\min_\leq$ and $\propname{TR}(\mathrm{S, \leq})$ there exists a $y \in \min_\leq(Y)$ such that $y < w$. But again by $\propname{TR}(\mathrm{S, \leq})$ this gives us $y < w < z$ which contradicts Eq~\ref{eq:lem_abs_minset_right_minsetY}.
\end{ind}
Hence
\begin{equation} \label{eq:lem_abs_minset_right_Y}
\forall y \in Y : \neg (y < z)
\end{equation}

Case $z \in X$
\begin{ind}
Then $z \in X \cup Y$, and by Eq~\ref{eq:lem_abs_minset_right_X} \& \ref{eq:lem_abs_minset_right_Y} we have that $\forall x \in X \cup Y : \neg (x < z)$. Therefore $z \in \min_\leq(X \cup Y)$.
\end{ind}

Case $z \in \min_\leq(Y)$
\begin{ind}
Then $z \in Y$ and hence $z \in X \cup Y$, and by Eq~\ref{eq:lem_abs_minset_right_X} \& \ref{eq:lem_abs_minset_right_Y} we have that $\forall x \in X \cup Y : \neg (x < z)$. Therefore $z \in \min_\leq(X \cup Y)$.
\end{ind}
Hence $z \in \min_\leq(X \cup \min_\leq(Y)) \Rightarrow z \in \min_\leq(X \cup Y)$.
\end{ind}

\vspace{1em}

Therefore $\min_\leq(X \cup \min_\leq(Y)) = \min_\leq(X \cup Y)$. 
\end{proof}


\vspace{2em}


\begin{lemma} \label{lem:minunion_right_absorption}
For all $X$ and $Y$:
\begin{equation}
\min_\leq(X \cup Y) = \min_\leq(X \cup \min_\leq(Y))
\end{equation}
\end{lemma}

\begin{proof}
Follows immediately from Lemma~\ref{lem:minunion_left_absorption} by the commutativity of $\cup$.
\end{proof}



\subsubsection{Associative}

\begin{theorem} \label{thm:minunion_as}
$\propname{AS}(\mathrm{MinUnion(S,\leq)}) \Leftrightarrow \propname{TRUE}$
\end{theorem}

\begin{proof}
Using Lemmas~\ref{lem:minunion_left_absorption}~\&~\ref{lem:minunion_right_absorption} we have:
\begin{align*}
X \minunion (Y \minunion Z) & = \min_\leq(X \cup \min_\leq(Y \cup Z)) \\
							& = \min_\leq(X \cup (Y \cup Z)) \\
							& = \min_\leq((X \cup Y) \cup Z) \\
							& = \min_\leq(\min_\leq(X \cup Y) \cup Z) \\
							& = (X \minunion Y) \minunion Z
\end{align*}
\end{proof}




\subsubsection{Identity}

\begin{theorem} \label{thm:minunion_id}
$\propname{ID}(\mathrm{MinUnion(S,\leq)}) \Leftrightarrow \propname{TRUE}$
\end{theorem}

\begin{proof}
Witness : $\emptyset$
\begin{align*}
X \minunion \emptyset 	& = \min_\leq(X \cup \emptyset) \\
						& = \min_\leq(X) \\
						& = X
\end{align*}

\begin{align*}
\emptyset \minunion X 	& = \min_\leq(\emptyset \cup X) \\
						& = \min_\leq(X) \\
						& = X
\end{align*}
\end{proof}




\subsubsection{Annihilator}

\begin{theorem} \label{thm:minunion_an}
$\propname{BM}(\mathrm{S,\leq}) \wedge \propname{AY}(\mathrm{S,\leq}) \Rightarrow (\propname{AN}(\mathrm{MinUnion(S,\leq)}) \Leftrightarrow \propname{TRUE})$
\end{theorem}


\begin{proof}
Witness: $\{\bot\}$

\begin{align*}
X \minunion \{\bot\} 	& = \min_\leq(X \cup \{\bot\}) \\
						& = \{\bot\}
\end{align*}

\begin{align*}
\{\bot\} \minunion X 	& = \min_\leq(\{\bot\} \cup X) \\
						& = \{\bot\}
\end{align*}
\end{proof}




\subsubsection{Commutative}

\begin{theorem} \label{thm:minunion_cm}
$\propname{CM}(\mathrm{MinUnion(S,\leq)}) \Leftrightarrow \propname{TRUE}$
\end{theorem}

\begin{proof}
Follows immediately from the commutativity of $\cup$:
\begin{align*}
X \minunion Y 	& = \min_\leq(X \cup Y) \\
				& = \min_\leq(Y \cup X) \\
				& = Y \minunion X
\end{align*}
\end{proof}




\subsubsection{Selective}

\begin{theorem} \label{thm:minunion_sl}
$\propname{SL}(\mathrm{MinUnion}(S,\leq)) \Leftrightarrow \propname{TO}(S,\leq)$
\end{theorem}

\begin{proof}
Assume $\propname{TO}(S,\leq)$.

\begin{ind}
Then every set can only contain a single element. Hence for all $x$ and $y$:
\begin{align*}
\{ x \} \minunion \{ y \} 	& = \min_\leq(\{ x \} \cup \{ y \}) \\
							& = \min_\leq(\{ x , y \}) 
\end{align*}
and as $x$ and $y$ are totally ordered, the result must either equal $\{ x \}$ or $\{ y \}$ and therefore we have that $\propname{SL}(\mathrm{MinUnion}(S,\leq))$.
\end{ind}

Assume $\neg \propname{TO}(S,\leq)$.

\begin{ind}
Then there exists $x$ and $y$ such that $x \nleq y$ and $y \nleq x$.
\begin{align*}
\{ x \} \minunion \{ y \} 	& = \min_\leq(\{ x \} \cup \{ y \}) \\
							& = \min_\leq(\{ x , y \}) \\
							& = \{ x , y \}
\end{align*}
Hence we have that $\neg \propname{SL}(\mathrm{MinUnion}(S,\leq))$.
\end{ind}
\end{proof}




\subsubsection{Idempotent}

\begin{theorem} \label{thm:minunion_ip}
$\propname{IP}(\mathrm{MinUnion(S,\leq)}) \Leftrightarrow \propname{TRUE}$
\end{theorem}

\begin{proof}
Follows immediately from the idempotence of $\cup$:
\begin{align*}
X \minunion X 	& = \min_\leq(X \cup X) \\
				& = \min_\leq(X) \\
				& = X
\end{align*}
\end{proof}



\subsubsection{IsLeft}

\begin{theorem} \label{thm:minunion_il}
$\propname{IL}(\mathrm{MinUnion(S,\leq)}) \Leftrightarrow \propname{FALSE}$
\end{theorem}

\begin{proof}
There exists an identity for $\mathrm{MinUnion(S,\leq)}$, therefore $\neg \propname{IL}(\mathrm{MinUnion(S,\leq)})$.
\end{proof}





\subsubsection{IsRight}

\begin{theorem} \label{thm:minunion_ir}
$\propname{IR}(\mathrm{MinUnion(S,\leq)}) \Leftrightarrow \propname{FALSE}$
\end{theorem}

\begin{proof}
There exists an identity for $\mathrm{MinUnion(S,\leq)}$, therefore $\neg \propname{IR}(\mathrm{MinUnion(S,\leq)})$.
\end{proof}





\subsubsection{LeftCancellative}

\begin{theorem} \label{thm:minunion_lc}
$\propname{LC}(\mathrm{MinUnion(S,\leq)}) \Leftrightarrow \propname{FALSE}$
\end{theorem}

\begin{proof}
There exists an identity for $\mathrm{MinUnion(S,\leq)}$, and at least two elements in $S$ and therefore two non-identity elements in ${\cal P}_{\mathrm{fin}}(S,\ \leq)$.
 
\vspace{0.5em}

Therefore $\neg \propname{LC}(\mathrm{MinUnion(S,\leq)})$.
\end{proof}




\subsubsection{RightCancellative}

\begin{theorem} \label{thm:minunion_rc}
$\propname{RC}(\mathrm{MinUnion(S,\leq)}) \Leftrightarrow \propname{FALSE}$
\end{theorem}

\begin{proof}
There exists an identity for $\mathrm{MinUnion(S,\leq)}$, and at least two elements in $S$ and therefore two non-identity elements in ${\cal P}_{\mathrm{fin}}(S,\ \leq)$. 

\vspace{0.5em}

Therefore $\neg \propname{RC}(\mathrm{MinUnion(S,\leq)})$.
\end{proof}





\subsubsection{LeftConstant}
\begin{theorem} \label{thm:minunion_lk}
$\propname{LK}(\mathrm{MinUnion(S,\leq)}) \Leftrightarrow \propname{FALSE}$
\end{theorem}

\begin{proof}
There exists an identity for $\mathrm{MinUnion(S,\leq)}$, therefore $\neg \propname{LK}(\mathrm{MinUnion(S,\leq)})$.
\end{proof}





\subsubsection{RightConstant}

\begin{theorem} \label{thm:minunion_rk}
$\propname{RK}(\mathrm{MinUnion(S,\leq)}) \Leftrightarrow \propname{FALSE}$
\end{theorem}

\begin{proof}
There exists an identity for $\mathrm{MinUnion(S,\leq)}$, therefore $\neg \propname{RK}(\mathrm{MinUnion(S,\leq)})$.
\end{proof}





\subsubsection{AntiLeft}

\begin{theorem} \label{thm:minunion_al}
$\propname{AL}(\mathrm{MinUnion(S,\leq)}) \Leftrightarrow \propname{FALSE}$
\end{theorem}


\begin{proof}
There exists an identity for $\mathrm{MinUnion(S,\leq)}$, therefore $\neg \propname{AL}(\mathrm{MinUnion(S,\leq)})$.
\end{proof}





\subsubsection{AntiRight}

\begin{theorem} \label{thm:minunion_ar}
$\propname{AR}(\mathrm{MinUnion(S,\leq)}) \Leftrightarrow \propname{FALSE}$
\end{theorem}

\begin{proof}
There exists an identity for $\mathrm{MinUnion(S,\leq)}$, therefore $\neg \propname{AR}(\mathrm{MinUnion(S,\leq)})$.
\end{proof}



\end{document}