
\begin{theorem} \label{thm:M_ld}
If $\propname{AY}(S,\otimes,\leq)$, $\propname{IP}(S,\otimes,\leq)$, $\propname{LI}(S,\otimes,\leq)$, $\propname{RI}(S,\otimes,\leq)$, $\propname{LM}(S,\otimes,\leq)$ and $\propname{RM}(S,\otimes,\leq)$ then
\begin{equation*}
\propname{LD}(\mathcal{M}(S,\ \otimes,\ \leq))  \Leftrightarrow \propname{TRUE}
\end{equation*}
\end{theorem}

\begin{proof}

\vspace{0.5em}
Consider arbitrary $X,Y,Z$
\begin{align*}
X \minunion (Y \minlift Z) 	& = \min_\leq(X \cup \min_\leq(Y \lift Z)) \\
							& = \min_\leq(X \cup (Y \lift Z)) & \text{(Lem \ref{lem:minunion_right_absorption})} \\
							& = \min_\leq(X \cup (X \lift Z) \cup (Y \lift X) \cup (Y \lift Z)) & \text{(Thm \ref{thm:N_lab} \& \ref{thm:N_rab})} \\
							& = \min_\leq((X \lift X) \cup (X \lift Z) \cup (Y \lift X) \cup (Y \lift Z)) & \text{(Thm \ref{thm:minlift_ip})} \\
							& = \min_\leq((X \cup Y) \lift (X \cup Z)) \\
							& = \min_\leq(\min_\leq(X \cup Y) \lift \min_\leq(X \cup Z)) & \text{(Lem \ref{lem:minlift_left_absorption} \& \ref{lem:minlift_right_absorption})} \\
							& = (X \minunion Y) \minlift (X \minunion Z)
\end{align*}
\end{proof}


\begin{theorem} \label{thm:M_rd}
If $\propname{AY}(S,\otimes,\leq)$, $\propname{IP}(S,\otimes,\leq)$, $\propname{LI}(S,\otimes,\leq)$, $\propname{RI}(S,\otimes,\leq)$, $\propname{LM}(S,\otimes,\leq)$ and $\propname{RM}(S,\otimes,\leq)$ then
\begin{equation*}
\propname{RD}(\mathcal{M}(S,\ \otimes,\ \leq))  \Leftrightarrow \propname{TRUE}
\end{equation*}
\end{theorem}

\begin{proof}

\vspace{0.5em}
Follows immediately from the proof of $\propname{LD}(\mathcal{M}(S,\ \otimes,\ \leq)$ by the commutativity of $\minunion$.
\end{proof}


\begin{theorem} \label{thm:M_za}
If $\propname{AY}(S,\leq)$, $\propname{BM}(S,\leq)$, $\propname{ID}(S,\otimes)$ and at least one of: $\propname{LI}(S,\ \leq,\ \otimes)$, $\propname{RI}(S,\ \leq,\ \otimes)$, $\propname{LM}(S,\ \leq,\ \otimes)$ or $\propname{RM}(S,\ \leq,\ \otimes)$ then
\begin{equation*}
\propname{ZA}(\mathcal{M}(S,\ \otimes,\ \leq)) \Leftrightarrow \propname{TRUE}
\end{equation*}
\end{theorem}

\begin{proof}

\vspace{0.5em}
Witness : $\{ \bot \}$

\vspace{0.5em}
Immediate from Theorem \ref{thm:N_oa}.
\end{proof}

\begin{theorem} \label{thm:M_oa}
$\propname{OA}(\mathcal{M}(S,\ \otimes,\ \leq)) \Leftrightarrow \propname{TRUE}$
\end{theorem}

\begin{proof}

\vspace{0.5em}
Witness : $\emptyset$

\vspace{0.5em}
Immediate from Theorem \ref{thm:N_za}.
\end{proof}

\begin{theorem} \label{thm:M_llab}
If $\propname{AY}(S,\otimes,\leq)$, $\propname{LI}(S,\otimes,\leq)$ and $\propname{RM}(S,\otimes,\leq)$ then
\begin{equation*}
\propname{LLAB}(\mathcal{N}(S,\otimes,\leq)) \Leftrightarrow \propname{TRUE}
\end{equation*}
\end{theorem}


\begin{proof}

\vspace{0.5em}
For all $X, Y$ we have
\begin{align*}
X \minlift (X \minunion Y) 	& = \min_\leq(X \lift \min_\leq(X \cup Y) ) \\
							& = \min_\leq( X \lift (X \cup Y)) & \text{(Lem \ref{lem:minlift_left_absorption})} \\
							& = \min_\leq(X \lift X \cup X \lift Y) \\
							& = \min_\leq(X \cup X \lift Y) & \text{(Thm \ref{thm:N_llab})} \\
							& = \min_\leq(X) \\
							& = X
\end{align*}
\end{proof}



\begin{theorem} \label{thm:M_lrab}
If $\propname{AY}(S,\otimes,\leq)$, $\propname{LI}(S,\otimes,\leq)$ and $\propname{RM}(S,\otimes,\leq)$ then
\begin{equation*}
\propname{LLAB}(\mathcal{N}(S,\otimes,\leq)) \Leftrightarrow \propname{TRUE}
\end{equation*}
\end{theorem}


\begin{proof}

\vspace{0.5em}
Immediately from Theorem~\ref{thm:M_llab} and the commutativity of $\minunion$.
\end{proof}



\begin{theorem} \label{thm:M_rlab}
If $\propname{AY}(S,\otimes,\leq)$, $\propname{RI}(S,\otimes,\leq)$ and $\propname{LM}(S,\otimes,\leq)$ then
\begin{equation*}
\propname{RLAB}(\mathcal{N}(S,\otimes,\leq)) \Leftrightarrow \propname{TRUE}
\end{equation*}
\end{theorem}


\begin{proof}

\vspace{0.5em}
For all $X, Y$ we have
\begin{align*}
(X \minunion Y) \minlift X 	& = \min_\leq(\min_\leq(X \cup Y) \lift X) \\
							& = \min_\leq((X \cup Y) \lift X) & \text{(Lem \ref{lem:minlift_right_absorption})} \\
							& = \min_\leq(X \lift X \cup Y \lift X) \\
							& = \min_\leq(X \cup Y \lift X) & \text{(Thm \ref{thm:N_rlab})} \\
							& = \min_\leq(X) \\
							& = X
\end{align*}
\end{proof}




\begin{theorem} \label{thm:M_rrab}
If $\propname{AY}(S,\otimes,\leq)$, $\propname{RI}(S,\otimes,\leq)$ and $\propname{LM}(S,\otimes,\leq)$ then
\begin{equation*}
\propname{RRAB}(\mathcal{N}(S,\otimes,\leq)) \Leftrightarrow \propname{TRUE}
\end{equation*}
\end{theorem}


\begin{proof}

\vspace{0.5em}
Immediately from Theorem~\ref{thm:M_rlab} and the commutativity of $\minunion$.
\end{proof}
